LogRel/STLC/Env.lean
@@ -10,3 +10,14 @@ def getr {α : Type} (x : ℕ) (l : List α) : Option α :=
 @[simp]
 def binds {α : Type} (x : ℕ) (a : α) (l : List α) :=
   getr x l = some a
+
+theorem getr_none {α : Type} : ∀ x (l : List α), x ≥ l.length → getr x l = none :=
+  by
+  intros x l HGe
+  induction l
+  case nil => rfl
+  case cons tail IH =>
+    simp at HGe
+    by_cases HEq : tail.length = x
+    . omega
+    . simp [if_neg HEq]; apply IH; omega
